Uppaal_Networks/AbsInt/State_Option.thy
@@ -57,77 +57,23 @@ end
 
 instantiation option :: (absstate) absstate
 begin
-definition "Sup_option (A::'a option set) = (if A = {} \<or> A = {\<bottom>} then \<bottom> else Some (\<Squnion>{x. Some x \<in> A}))"
-definition "Inf_option (A::'a option set) = (if None \<in> A then None else Some (\<Sqinter>{x. Some x \<in> A}))"
 instance proof (standard, goal_cases)
-  case (1 x y) then show ?case by (cases x; cases y) auto
+  case (1 x y)
+then show ?case sorry
 next
-  case (2 x y) then show ?case by (cases x; cases y) auto
+  case (2 y x)
+then show ?case sorry
 next
-  case (3 x y z) then show ?case by (cases x; cases y; cases z) auto
+  case (3 y x z)
+  then show ?case sorry
 next
-  case (4 x y) then show ?case by (cases x; cases y) auto
+  case (4 a)
+  then show ?case sorry
 next
-  case (5 y x) then show ?case by (cases x; cases y) auto
-next
-  case (6 y x z) then show ?case by (cases x; cases y; cases z) auto
-next
-  case (7 x A)
-  then show ?case
-  proof (cases x)
-    case None then show ?thesis using 7 by (simp add: Inf_option_def)
-  next
-    case (Some a) then show ?thesis using 7 by (simp add: Inf_lower Inf_option_def)
-  qed
-next
-  case (8 A z)
-  then show ?case
-  proof (cases z)
-    case (Some a)
-    then show ?thesis using 8 Inf_option_def le_Inf_iff
-      by (metis (mono_tags, lifting) less_eq_option.simps(3) mem_Collect_eq)
-  qed simp
-next
-  case (9 x A)
-  then show ?case
-  proof (cases "A = {} \<or> A = {\<bottom>}")
-    case True
-    then show ?thesis using "9" bot_option_def by auto
-  next
-    case False
-    have "x \<le> Some (\<Squnion>{x. Some x \<in> A})"
-    proof(cases x)
-      case (Some a)
-      then show ?thesis by (metis 9 Sup_upper less_eq_option.simps(3) mem_Collect_eq)
-    qed simp
-    from False this show ?thesis by (simp add: Sup_option_def)
-  qed
-next
-  case (10 A z)
-  then show ?case
-  proof (cases "A = {} \<or> A = {\<bottom>}")
-    case True
-    then show ?thesis by (simp add: Sup_option_def)
-  next
-    case False
-    then show ?thesis
-    proof(cases z)
-      case None
-      then show ?thesis using "10" False bot_option_def dual_order.antisym by fastforce
-    next
-      case (Some a)
-      then show ?thesis by (metis (mono_tags, lifting) "10" False Sup_le_iff Sup_option_def less_eq_option.simps(3) mem_Collect_eq)
-    qed
-  qed
-next
-  case 11 then show ?case by (simp add: Inf_option_def)
-next
-  case 12 then show ?case by (simp add: Sup_option_def)
+  case (5 a)
+  then show ?case sorry
 qed
 end
-
-lemma[code]: "Sup ((set A)::('a::absstate) option set) = fold sup A \<bottom>" by (rule List.complete_lattice_class.Sup_set_fold)
-lemma[code]: "Inf ((set A)::('a::absstate) option set) = fold inf A \<top>" by (rule List.complete_lattice_class.Inf_set_fold)
 
 fun \<gamma>_option :: "('a \<Rightarrow> 'b set) \<Rightarrow> 'a option \<Rightarrow> 'b set" where
 "\<gamma>_option \<gamma> None = {}" |
